Advanced proof of p2b on id = id2 case

Distributed/Paxos/p2b.lean
@@ -2,6 +2,7 @@ import Distributed.base_structures
 import Distributed.Paxos.paxos_model
 import Distributed.Paxos.p2c
 import Distributed.Paxos.learner_helpers
+import Distributed.Paxos.acceptors_helpers
 import Mathlib.Tactic.ByContra
 import Mathlib.Tactic.Cases 
 
@@ -10,24 +11,37 @@ open PaxosModel
 namespace PaxosProof
 
 
--- INV4b1
 
+
+
+-- INV4b1
 def inv4b1 (s: System a l p) (i: Fin a) (v: Value) (id: PropId) :=
 Message.Learn (i,  v, id)  ∈ s.network.messages
 -> ∀  id' p, Message.Promise id' i p ∈ s.network.messages
--> id' >= id
+-> id' > id
 -> p ≠ none
-
-
 
 theorem inv4b1Proof_ind (s1 s2: System a l p) (i: Fin a)  (v: Value) (id: PropId) :
 step s1 s2
 -> inv4b1 s1 i v id
--> inv41  s1 i v id
--> (∀ i, (s1.acceptors i).id = i)
+-> inv41 s1 i v id
+-> (∀ k, (s1.acceptors k).id = k)
 -> inv4b1 s2 i v id := by
-   simp [inv4b1]; intros step IH i41 iEq i4b2 mLearn id2 prop  mProp id2Boun
-   sorry
+   simp [inv4b1]; intros step IH i41 idIsK mLearnInN id' opt mPromisInN idBound
+   cases step <;> rename_i stepRule <;> cases stepRule <;> repeat (rename_i stepRule; rcases stepRule) <;> (try grind)
+   . simp at *; rename_i j pid mess acc net accNat netNat mRules
+     subst accNat; rw [netNat] at mLearnInN mPromisInN; simp at mLearnInN mPromisInN
+     cases mPromisInN <;> try grind
+     rename_i eqs; rcases eqs with ⟨ eq1, eq2, eq3 ⟩; subst_vars
+     have ⟨ v', id' , idBound, sAccSome ⟩  := i41 mLearnInN
+     rw [idIsK j] at sAccSome; rw [sAccSome]; simp
+   . simp at *; rename_i mNat; rw [mNat] at mLearnInN mPromisInN; simp at mLearnInN mPromisInN; rename_i j net v2 pid accSome
+     cases mLearnInN <;> try grind
+     rename_i eqs; rcases eqs with ⟨ e1, e2, e3 ⟩; subst e1 e2 e3
+     by_cases c:(opt = none) <;> try grind
+     subst c; simp; clear mNat
+     sorry
+
 theorem inv4b1Proof (s: System a l p) (i: Fin a) (v: Value) (id: PropId)  :
 systemIsValid s
 -> inv4b1 s i v id:= by
@@ -45,6 +59,12 @@ induction s0Steps  with
   sorry
 
 
+
+
+
+
+
+
 -- INV4b
 def inv4b (s: System a l p) (v : Value) (id: PropId) :=
 (∃ set, count set > a / 2 ∧ (∀ (i: Fin a), contains  set i -> Message.Learn (i, v, id) ∈ s.network.messages))
@@ -56,17 +76,14 @@ def inv4b (s: System a l p) (v : Value) (id: PropId) :=
 theorem inv4bProof (s: System a l p) (v: Value) (id: PropId)  :
 systemIsValid s
 -> inv4b s v id:= by
-intros sIsValid setRule id2 v2 mAccs
+intros sIsValid setRule id2 v2 mAccs idBound
 rcases setRule with ⟨ set1, setCount1, setContains1 ⟩ 
 have ⟨ set2, setCount2, setContains2R1, setContains2R2 ⟩  := inv4cProof s v2 id2 sIsValid mAccs
 have ⟨ i, iContained1, iContained2 ⟩ := setMaxContainsBoth set1 set2 setCount1 setCount2
-rcases setContains2R2 with setContains2R2 | setContains2R3
-. have p1 := setContains2R2 i iContained2
-  have p2 := setContains1 i iContained1
-  intros id2Bound; exfalso
-  have dd := inv4b1Proof s i v id sIsValid p2 id2 none p1 id2Bound (by simp)
-  exact dd
-. rcases setContains2R3 with ⟨ existsOneId, forAllId ⟩ 
-  have p2 := setContains1 i iContained1
-  have ⟨ prop , p3 ⟩ := setContains2R1 i iContained2
-  sorry
+by_cases (id2 = id)
+. rename_i eq; subst eq
+  have l1 := setContains1 i iContained1
+  have ⟨ p, l2 ⟩  := setContains2R1 i iContained2
+  have i3 := inv3Proof s i v id2 sIsValid l1
+  rw [inva1Proof s v2 v id2 sIsValid mAccs i3]
+. sorry
