Distributed/Paxos/acceptors_helpers.lean
@@ -1,0 +1,78 @@
+import Distributed.base_structures
+import Distributed.Paxos.paxos_model
+import Mathlib.Tactic.ByContra
+import Mathlib.Tactic.Cases 
+
+open Model
+open PaxosModel
+namespace PaxosProof
+
+def inva4 (s: System a l p)  (j c: Fin p) :=
+(s.proposers j).propId = (s.proposers c).propId
+-> j = c
+
+
+def inva3 (s: System a l p) (j: Fin p) :=
+count (s.proposers j).propRec ≤ a / 2
+-> ∀ v, Message.Accept ((s.proposers j).propId, v) ∉ s.network.messages
+
+
+
+--INVA2
+def inva2 (s: System a l p) (v: Value) (j: Fin p) :=
+Message.Accept ((s.proposers j).propId, v) ∈ s.network.messages
+-> a / 2 < count (s.proposers j).propRec
+->  (s.proposers j).propVal = some v
+
+
+
+theorem inva2Proof_ind (s1 s2: System a l p) (v: Value) (id: PropId) (j: Fin p) :
+step s1 s2
+-> inva2 s1 v j
+-> (∀ j, inva3 s1 j)
+-> (∀ i j, inva4 s1 i j)
+-> inva2 s2 v j := by
+simp [inva2]; intros step IH ia3 ia4 MAccInN countProp
+cases step <;> rename_i stepRule <;> cases stepRule <;> (try (rename_i stepRule; simp at stepRule; grind))  <;> repeat (rename_i stepRule; rcases stepRule) <;> subst_vars
+. simp [updateMap] at *; split <;> try grind
+  rename_i eq; subst eq;simp at countProp
+  rw [emptySetEqZero] at countProp
+  omega
+. rename_i i accId prop opt v1 pid  mInN idBound countBound noneImpX splitX 
+  simp [updateMap] at * <;> split at MAccInN <;> split at splitX <;> subst splitX <;> rename_i a b <;> have contra := ia3 i countBound v <;> (try subst a) <;> (try simp [contra] at MAccInN) <;> try grind  
+. rename_i a b c d e ;simp [updateMap] at *; split
+  . split at e <;> try grind
+  . rename_i neq; simp [neq] at *; clear neq;
+    sorry
+    
+      
+      
+    
+  
+  
+
+
+
+--INVA1
+def inva1 (s: System a l p) (v1 v2: Value) (id: PropId):=
+Message.Accept (id, v1) ∈ s.network.messages
+-> Message.Accept (id, v2) ∈ s.network.messages
+-> v1 = v2
+
+
+theorem inva1Proof_ind (s1 s2: System a l p) (v1 v2: Value) (id: PropId) :
+step s1 s2
+-> inva1 s1 v1 v2 id
+-> (∀ v j, inva2 s2 v j)
+-> inva1 s2 v1 v2 id := by
+simp [inva1]; intros step IH ia2 m1InN m2InN
+cases step <;> rename_i stepRule <;> cases stepRule <;> try (rename_i stepRule; simp at stepRule; grind)
+. simp at *; rename_i prop v net j stepRule;
+  rcases stepRule with ⟨ bound,pNat, rest ⟩ ; subst pNat
+  have c1 := ia2 v1 j ; have c2 := ia2 v2 j; simp [inva2, updateMap] at c1 c2; grind   
+
+
+  
+theorem inva1Proof (s: System a l p) (v1 v2: Value) (id: PropId) :
+systemIsValid s
+-> inva1 s v1 v2 id := by sorry
